michael_formal/not4afp/Paper_Example.thy
@@ -1,5 +1,5 @@
 theory Paper_Example
-imports Inference SelectionStrategies FSet_Utils
+imports Inference SelectionStrategies
 begin
 
 definition select :: transition where
@@ -85,917 +85,146 @@ lemma coin50_posterior: "posterior \<lbrakk>V (R 1) \<mapsto> cexp.Bc True\<rbra
   apply clarify
   by (simp add: consistent_empty_4)
 
-definition drinks_before :: transition_matrix where
-  "drinks_before = {|((0, 1), select), ((1, 2), coin50), ((2, 2), coin), ((2, 2), vend_fail), ((2, 3), vend_success)|}"
+definition drinks_before :: iEFSM where
+  "drinks_before = {|(0, (0, 1), select), (1, (1, 2), coin50), (2, (2, 2), coin), (3, (2, 2), vend_fail), (4, (2, 3), vend_success)|}"
 
-definition drinks_after :: transition_matrix where
-  "drinks_after = {|((0, 1), select_update), ((1, 1), coin), ((1, 1), vend_fail), ((1, 3), vend_success)|}"
+definition drinks_after :: iEFSM where
+  "drinks_after = {|(0, (0, 1), select_update), (1, (1, 1), coin), (2, (1, 1), vend_fail), (3, (1, 3), vend_success)|}"
 
-definition merge_1_2 :: transition_matrix where
-  "merge_1_2 = {|((0, 1), select), ((1, 1), coin50), ((1, 1), coin), ((1, 1), vend_fail), ((1, 3), vend_success)|}"
-
-lemma merge_1_2: "merge_states 1 2 drinks_before = merge_1_2"
-  by (simp add: merge_states_def drinks_before_def merge_1_2_def merge_states_aux_def)
-
-definition merge_1_2_update :: transition_matrix where
-  "merge_1_2_update = {|((0, 1), select_update), ((1, 1), coin50), ((1, 1), coin), ((1, 1), vend_fail), ((1, 3), vend_success)|}"
+definition merge_1_2_update :: iEFSM where
+  "merge_1_2_update = {|(0, (0, 1), select_update), (1, (1, 1), coin50), (2, (1, 1), coin), (3, (1, 1), vend_fail), (4, (1, 3), vend_success)|}"
 
 definition update_mapping :: "nat \<Rightarrow> nat" where
   "update_mapping x = x"
 
-lemma possible_steps_drinks_before_select: "length b = 1 \<Longrightarrow> possible_steps drinks_before 0 r ''select'' b = {|(1, select)|}"
-proof-
-  assume premise: "length b = 1"
-  have set_filter: "(Set.filter
-       (\<lambda>((origin, dest), t).
-           origin = 0 \<and>
-           Label t = ''select'' \<and> length b = Arity t \<and> apply_guards (Guard t) (case_vname (\<lambda>n. input2state b 1 (I n)) (\<lambda>n. r (R n))))
-       (fset drinks_before)) = {((0, 1), select)}"
-    apply (simp add: Set.filter_def drinks_before_def)
-    apply safe
-    by (simp_all add: transitions premise)
-  show ?thesis
-    by (simp add: possible_steps_def ffilter_def set_filter)
-qed
-
-lemma possible_steps_merge_1_2_select: "length b = 1 \<Longrightarrow> possible_steps merge_1_2 0 r ''select'' b = {|(1, select)|}"
-proof-
-  assume premise: "length b = 1"
-  have set_filter: "(Set.filter
-       (\<lambda>((origin, dest), t).
-           origin = 0 \<and>
-           Label t = ''select'' \<and> length b = Arity t \<and> apply_guards (Guard t) (case_vname (\<lambda>n. input2state b 1 (I n)) (\<lambda>n. r (R n))))
-       (fset merge_1_2)) =
-    {((0, 1), select)}"
-    apply (simp add: merge_1_2_def Set.filter_def)
-    apply safe
-    by (simp_all add: transitions premise)
-  show ?thesis
-    by (simp add: possible_steps_def ffilter_def set_filter)
-qed
-
-lemma possible_steps_merge_1_2_update_select: "length b = 1 \<Longrightarrow> possible_steps merge_1_2_update 0 r ''select'' b = {|(1, select_update)|}"
-proof-
-  assume premise: "length b = 1"
-  have set_filter: "(Set.filter
-       (\<lambda>((origin, dest), t).
-           origin = 0 \<and>
-           Label t = ''select'' \<and> length b = Arity t \<and> apply_guards (Guard t) (case_vname (\<lambda>n. input2state b 1 (I n)) (\<lambda>n. r (R n))))
-       (fset merge_1_2_update)) =
-    {((0, 1), select_update)}"
-    apply (simp add: Set.filter_def merge_1_2_update_def)
-    apply safe
-    by (simp_all add: transitions premise)
-  show ?thesis
-    by (simp add: possible_steps_def ffilter_def set_filter)
-qed
-
-lemma drinks_before_step_0_invalid: "\<not> (aa = ''select'' \<and> length b = 1) \<Longrightarrow>
-        nondeterministic_step drinks_before 0 Map.empty aa b = None"
-proof-
-  assume premise: "\<not> (aa = ''select'' \<and> length b = 1)"
-  have set_filter: "(Set.filter
-           (\<lambda>((origin, dest), t).
-               origin = 0 \<and> Label t = aa \<and> length b = Arity t \<and> apply_guards (Guard t) (case_vname (\<lambda>n. input2state b 1 (I n)) Map.empty))
-           (fset drinks_before)) = {}"
-    apply (simp add: Set.filter_def drinks_before_def)
-    apply safe
-    using premise
-    by (simp_all add: transitions)
-  show ?thesis
-    by (simp add: nondeterministic_step_def possible_steps_def ffilter_def set_filter)
-qed
-
-lemma possible_steps_drinks_before_coin_50: "possible_steps drinks_before 1 r ''coin'' [Num 50] = {|(2, coin50)|}"
-proof-
-  have set_filter: "(Set.filter
-       (\<lambda>((origin, dest), t).
-           origin = 1 \<and>
-           Label t = ''coin'' \<and> Suc 0 = Arity t \<and> apply_guards (Guard t) (case_vname (\<lambda>n. input2state [Num 50] 1 (I n)) (\<lambda>n. r (R n))))
-       (fset drinks_before)) =
-    {((1, 2), coin50)}"
-    apply (simp add: drinks_before_def Set.filter_def)
-    apply safe
-    by (simp_all add: transitions)
-  have abs_fset: "Abs_fset {((1, 1), coin50), ((1, 1), coin)} = {|((1, 1), coin50), ((1, 1), coin)|}"
-    by (metis finsert.rep_eq fset_inverse fset_simps(1))
-   show ?thesis
-     by (simp add: possible_steps_def ffilter_def set_filter abs_fset)
- qed
-
-lemma drinks_before_1_invalid: "\<not> (aa = ''coin'' \<and> b = [Num 50]) \<Longrightarrow> nondeterministic_step drinks_before 1 r aa b = None"
-proof-
-  assume premise: "\<not>(aa = ''coin'' \<and> b = [Num 50])"
-  have set_filter: "(Set.filter
-           (\<lambda>((origin, dest), t).
-               origin = 1 \<and>
-               Label t = aa \<and> length b = Arity t \<and> apply_guards (Guard t) (case_vname (\<lambda>n. input2state b 1 (I n)) (\<lambda>n. r (R n))))
-           (fset drinks_before)) = {}"
-    using premise
-    apply (simp add: drinks_before_def Set.filter_def coin50_def)
-    by (metis One_nat_def input2state.simps(2) length_0_conv length_Suc_conv option.inject)
-  show ?thesis
-    by (simp add: nondeterministic_step_def possible_steps_def ffilter_def set_filter)
-qed
-
-lemma merge_1_2_invalid_coin_input: "aa = ''coin'' \<Longrightarrow> length b \<noteq> 1 \<Longrightarrow> nondeterministic_step merge_1_2 1 <R 1 := d> ''coin'' b = None"
-proof-
-  assume premise1: "aa = ''coin''"
-  assume premise2: "length b \<noteq> 1"
-  have set_filter: "(Set.filter
-           (\<lambda>((origin, dest), t).
-               origin = 1 \<and>
-               Label t = ''coin'' \<and>
-               length b = Arity t \<and> apply_guards (Guard t) (case_vname (\<lambda>n. input2state b 1 (I n)) (\<lambda>n. if n = 1 then Some d else None)))
-           (fset merge_1_2)) = {}"
-    using premise1 premise2
-    apply (simp add: merge_1_2_def Set.filter_def)
-    apply safe
-    by (simp_all add: transitions)
-  show ?thesis
-    by (simp add: nondeterministic_step_def possible_steps_def ffilter_def set_filter)
-qed
-
-lemma merge_1_2_possible_steps_coin_not_50: "aa = ''coin'' \<Longrightarrow>
-    length b = 1 \<Longrightarrow>
-    b \<noteq> [Num 50] \<Longrightarrow>
-    possible_steps merge_1_2 1 <R 1 := d> ''coin'' b = {|(1, coin)|}"
-proof-
-  assume premise1: "aa = ''coin''"
-  assume premise2: "length b = 1"
-  assume premise3: "b \<noteq> [Num 50]"
-  have set_filter: "(Set.filter
-       (\<lambda>((origin, dest), t).
-           origin = 1 \<and>
-           Label t = ''coin'' \<and> length b = Arity t \<and> apply_guards (Guard t) (case_vname (\<lambda>n. input2state b 1 (I n)) (\<lambda>n. <R 1 := d> (R n))))
-       (fset merge_1_2)) = {((1, 1), coin)}"
-    using premise1 premise2 premise3
-    apply (simp add: merge_1_2_def Set.filter_def)
-    apply safe
-           apply (simp_all add: transitions)
-    by (metis One_nat_def input2state.simps(2) length_0_conv length_Suc_conv option.inject)
-  show ?thesis
-    by (simp add: possible_steps_def ffilter_def set_filter)
-qed
-
-lemma merge_1_2_update_possible_steps_coin_50: "possible_steps merge_1_2_update 1 <R 1 := d, R 2 := Num n> ''coin'' [Num 50] = {|(1, coin50), (1, coin)|}"
-proof-
-  have set_filter: "(Set.filter
-       (\<lambda>((origin, dest), t).
-           origin = 1 \<and>
-           Label t = ''coin'' \<and>
-           Suc 0 = Arity t \<and> apply_guards (Guard t) (case_vname (\<lambda>n. input2state [Num 50] 1 (I n)) (\<lambda>na. <R 1 := d, R 2 := Num n> (R na))))
-       (fset merge_1_2_update)) = {((1, 1), coin), ((1, 1), coin50)}"
-    apply (simp add: Set.filter_def merge_1_2_update_def)
-    apply safe
-    by (simp_all add: transitions)
-  have abs_fset: "Abs_fset {((1, 1), coin), ((1, 1), coin50)} = {|((1, 1), coin), ((1, 1), coin50)|}"
-    by (metis finsert.rep_eq fset_inverse fset_simps(1))
-  show ?thesis
-    apply (simp add: possible_steps_def ffilter_def set_filter abs_fset)
-    by auto
-qed
-
-lemma possible_steps_drinks_before_coin: "length b = 1 \<Longrightarrow> possible_steps drinks_before 2 r1 ''coin'' b = {|(2, coin)|}"
-proof-
-  assume premise: "length b = 1"
-  have set_filter: "(Set.filter
-       (\<lambda>((origin, dest), t).
-           origin = 2 \<and>
-           Label t = ''coin'' \<and> length b = Arity t \<and> apply_guards (Guard t) (case_vname (\<lambda>n. input2state b 1 (I n)) (\<lambda>n. r1 (R n))))
-       (fset drinks_before)) = {((2, 2), coin)}"
-    apply (simp add: drinks_before_def Set.filter_def)
-    apply safe
-    by (simp_all add: transitions premise)
-  show ?thesis
-    by (simp add: possible_steps_def ffilter_def set_filter)
-qed
-
-lemma possible_steps_merge_1_2_update_coin: "length b = 1 \<Longrightarrow> (1, coin) |\<in>| possible_steps merge_1_2_update 1 r2 ''coin'' b"
-proof-
-  assume premise: "length b = 1"
-  have set_filter: "((1, 1), coin) \<in> (Set.filter
-       (\<lambda>((origin, dest), t).
-           origin = 1 \<and>
-           Label t = ''coin'' \<and> length b = Arity t \<and> apply_guards (Guard t) (case_vname (\<lambda>n. input2state b 1 (I n)) (\<lambda>n. r2 (R n))))
-       (fset merge_1_2_update))"
-    apply (simp add: merge_1_2_update_def Set.filter_def)
-    apply safe
-    by (simp_all add: transitions premise)
-  show ?thesis
-    apply (simp add: possible_steps_def ffilter_def)
-    using set_filter
-    by (metis (no_types, lifting) case_prod_conv ffilter.rep_eq fimage_eqI fset_inverse notin_fset)
-qed
-
-lemma nondeterministic_step_drinks_before_invalid_step_2: " \<not> (aa = ''coin'' \<and> length b = 1) \<Longrightarrow>
-       \<not> (aa = ''vend'' \<and> b = []) \<Longrightarrow> nondeterministic_step drinks_before 2 r1 aa b = None"
-proof-
-  assume premise1:  "\<not> (aa = ''coin'' \<and> length b = 1)"
-  assume premise2: "\<not> (aa = ''vend'' \<and> b = [])"
-  have set_filter: "(Set.filter
-           (\<lambda>((origin, dest), t).
-               origin = 2 \<and>
-               Label t = aa \<and> length b = Arity t \<and> apply_guards (Guard t) (case_vname (\<lambda>n. input2state b 1 (I n)) (\<lambda>n. r1 (R n))))
-           (fset drinks_before)) = {}"
-    using premise1 premise2
-    apply (simp add: Set.filter_def drinks_before_def)
-    apply safe
-    by (simp_all add: transitions)
-  show ?thesis
-    by (simp add: nondeterministic_step_def possible_steps_def ffilter_def set_filter)
-qed
-
-lemma impossible_steps_drinks_before_vend: "\<nexists>n. r (R 2) = Some (Num n) \<Longrightarrow> nondeterministic_step drinks_before 2 r ''vend'' i = None"
-proof-
-  assume premise: "\<nexists>n. r (R 2) = Some (Num n)"
-  have set_filter: "(Set.filter
-       (\<lambda>((origin, dest), t).
-           origin = 2 \<and>
-           Label t = ''vend'' \<and> length i = Arity t \<and> apply_guards (Guard t) (case_vname (\<lambda>n. input2state i 1 (I n)) (\<lambda>n. r (R n))))
-       (fset drinks_before)) = {}"
-    using premise
-    apply (simp add: Set.filter_def drinks_before_def)
-    apply safe
-      apply (simp add: transitions)
-     apply (simp add: transitions)
-     apply (metis MaybeBoolInt.elims option.simps(3))
-     apply (simp add: transitions)
-    apply (case_tac "MaybeBoolInt (\<lambda>x y. y < x) (Some (Num 100)) (r (R 2))")
-     apply simp
-    apply simp
-    by (metis MaybeBoolInt.elims option.simps(3))
-  show ?thesis
-    by (simp add: nondeterministic_step_def possible_steps_def ffilter_def set_filter)
-qed
-
-lemma drinks_before_vend_fail: "r (R 2) = Some (Num x1) \<Longrightarrow> x1 < 100 \<Longrightarrow> possible_steps drinks_before 2 r ''vend'' [] = {|(2, vend_fail)|}"
-proof-
-  assume premise1: "r (R 2) = Some (Num x1)"
-  assume premise2: "x1 < 100"
-  have set_filter: "(Set.filter
-       (\<lambda>((origin, dest), t).
-           origin = 2 \<and> Label t = ''vend'' \<and> Arity t = 0 \<and> apply_guards (Guard t) (case_vname (\<lambda>n. input2state [] 1 (I n)) (\<lambda>n. r (R n))))
-       (fset drinks_before)) = {((2, 2), vend_fail)}"
-    using premise1 premise2
-    apply (simp add: Set.filter_def drinks_before_def)
-    apply safe
-    by (simp_all add: transitions)
-  show ?thesis
-    by (simp add: possible_steps_def ffilter_def set_filter)
-qed
-
-lemma drinks_before_vend_success: "r (R 2) = Some (Num x1) \<Longrightarrow> x1 \<ge> 100 \<Longrightarrow> possible_steps drinks_before 2 r ''vend'' [] = {|(3, vend_success)|}"
-proof-
-  assume premise1: "r (R 2) = Some (Num x1)"
-  assume premise2: "x1 \<ge> 100"
-  have set_filter: "(Set.filter
-       (\<lambda>((origin, dest), t).
-           origin = 2 \<and> Label t = ''vend'' \<and> Arity t = 0 \<and> apply_guards (Guard t) (case_vname (\<lambda>n. input2state [] 1 (I n)) (\<lambda>n. r (R n))))
-       (fset drinks_before)) = {((2, 3), vend_success)}"
-    using premise1 premise2
-    apply (simp add: Set.filter_def drinks_before_def)
-    apply safe
-    by (simp_all add: transitions)
-  show ?thesis
-    by (simp add: possible_steps_def ffilter_def set_filter)
-qed
-
-lemma merge_1_2_update_vend_fail: "r (R 2) = Some (Num x1) \<Longrightarrow> x1 < 100 \<Longrightarrow> possible_steps merge_1_2_update 1 r ''vend'' [] = {|(1, vend_fail)|}"
-  proof-
-  assume premise1: "r (R 2) = Some (Num x1)"
-  assume premise2: "x1 < 100"
-  have set_filter: "(Set.filter
-       (\<lambda>((origin, dest), t).
-           origin = 1 \<and> Label t = ''vend'' \<and> Arity t = 0 \<and> apply_guards (Guard t) (case_vname (\<lambda>n. input2state [] 1 (I n)) (\<lambda>n. r (R n))))
-       (fset merge_1_2_update)) = {((1, 1), vend_fail)}"
-    using premise1 premise2
-    apply (simp add: Set.filter_def merge_1_2_update_def)
-    apply safe
-    by (simp_all add: transitions)
-  show ?thesis
-    by (simp add: possible_steps_def ffilter_def set_filter)
-qed
-
-lemma merge_1_2_update_vend_success: "r (R 2) = Some (Num x1) \<Longrightarrow> x1 \<ge> 100 \<Longrightarrow> possible_steps merge_1_2_update 1 r ''vend'' [] = {|(3, vend_success)|}"
-  proof-
-  assume premise1: "r (R 2) = Some (Num x1)"
-  assume premise2: "x1 \<ge> 100"
-  have set_filter: "(Set.filter
-       (\<lambda>((origin, dest), t).
-           origin = 1 \<and> Label t = ''vend'' \<and> Arity t = 0 \<and> apply_guards (Guard t) (case_vname (\<lambda>n. input2state [] 1 (I n)) (\<lambda>n. r (R n))))
-       (fset merge_1_2_update)) = {((1, 3), vend_success)}"
-    using premise1 premise2
-    apply (simp add: merge_1_2_update_def Set.filter_def)
-    apply safe
-    by (simp_all add: transitions)
-  show ?thesis
-    by (simp add: possible_steps_def ffilter_def set_filter)
-qed
-
-lemma drinks_before_ends_at_3: "nondeterministic_step drinks_before 3 r aa b = None"
-proof-
-  have set_filter: "(Set.filter
-           (\<lambda>((origin, dest), t).
-               origin = 3 \<and>
-               Label t = aa \<and> length b = Arity t \<and> apply_guards (Guard t) (case_vname (\<lambda>n. input2state b 1 (I n)) (\<lambda>n. r (R n))))
-           (fset drinks_before)) = {}"
-    by (simp add: drinks_before_def Set.filter_def)
-  show ?thesis
-    by (simp add: nondeterministic_step_def possible_steps_def ffilter_def set_filter)
-qed
-
 definition update_before :: "nat \<Rightarrow> nat" where
   "update_before x = (if x = 2 then 1 else x)"
 
-lemma simulation_2_1: "\<forall>r. nondeterministic_simulates_trace merge_1_2_update drinks_before 1 2 r r lst update_before"
-proof (induct lst)
-  case Nil
-  then show ?case
-    by (simp add: nondeterministic_simulates_trace.base)
-next
-  case (Cons a lst)
-  then show ?case
-    apply (case_tac a)
-    apply simp
-     apply (rule allI)
-    apply (case_tac "aa = ''coin'' \<and> length b = 1")
-     apply simp
-     apply (rule nondeterministic_simulates_trace.step_some)
-         apply (simp add: update_before_def)
-        apply (simp add: nondeterministic_step_def possible_steps_drinks_before_coin)
-    using possible_steps_merge_1_2_update_coin
-       apply blast
-      apply simp
-     apply simp
-    apply (case_tac "aa = ''vend'' \<and> b = []")
-     defer
-     apply (rule nondeterministic_simulates_trace.step_none)
-    using nondeterministic_step_drinks_before_invalid_step_2
-     apply blast
-    apply simp
-    apply (case_tac "r (R 2)")
-     apply (rule nondeterministic_simulates_trace.step_none)
-     apply (simp add: impossible_steps_drinks_before_vend)
-    apply (case_tac aaa)
-     defer
-     apply (rule nondeterministic_simulates_trace.step_none)
-     apply (simp add: impossible_steps_drinks_before_vend)
-    apply clarify
-    apply simp
-    apply (case_tac "x1 < 100")
-     apply (rule nondeterministic_simulates_trace.step_some)
-         apply (simp add: update_before_def)
-        apply (simp add: nondeterministic_step_def drinks_before_vend_fail)
-       apply (simp add: merge_1_2_update_vend_fail)
-      apply simp
-     apply (simp add: vend_fail_def)
-    apply (rule nondeterministic_simulates_trace.step_some)
-        apply (simp add: update_before_def)
-       apply (simp add: nondeterministic_step_def drinks_before_vend_success)
-      apply (simp add: merge_1_2_update_vend_success)
-     apply simp
-    apply (simp add: vend_success_def)
-    apply (case_tac lst)
-     apply (simp add: nondeterministic_simulates_trace.base)
-    apply simp
-    apply clarify
-    apply (rule nondeterministic_simulates_trace.step_none)
-    by (simp add: drinks_before_ends_at_3)
-  qed
+definition modifier :: update_modifier where
+  "modifier a b c d e =  Some (merge_1_2_update, update_mapping, update_before)"
 
-lemma simulation_1_1: "nondeterministic_simulates_trace merge_1_2_update drinks_before 1 1 <R 1 := d, R 2 := Num 0> <R 1 := d> ((aa, b) # list) update_before"
+lemma scoring_1: "sorted_list_of_fset (score drinks_before naive_score) = [(0, 0, 1), (0, 0, 2), (0, 0, 3), (0, 1, 3), (0, 2, 3), (1, 1, 2)]"
 proof-
-  have choice_coin50_coin: "(\<exists>a b. a = 1 \<and> b = coin50 \<or> a = 1 \<and> b = coin)"
+  have S_drinks_before: "S drinks_before = {|0, 1, 2, 3|}"
+    apply (simp add: S_def drinks_before_def)
     by auto
-  have coin50_updates: "(EFSM.apply_updates (Updates coin50)
-       (case_vname (\<lambda>n. if n = 1 then Some (Num 50) else input2state [] (1 + 1) (I n)) (\<lambda>n. if n = 1 then Some d else None)) <R 1 := d>) = 
-        <R 1 := d, R 2 := Num 50>"
-    apply (rule ext)
-    by (simp add: coin50_def)
-  have coin50_updates_2: "(EFSM.apply_updates (Updates coin50) (\<lambda>x. case x of I n \<Rightarrow> input2state [Num 50] 1 (I n) | R n \<Rightarrow> <R 1 := d, R 2 := Num 0> (R n))
-       <R 1 := d, R 2 := Num 0>) = <R 1 := d, R 2 := Num 50>"
-    apply (rule ext)
-    by (simp add: coin50_def)
-  have set_filter: "\<forall>b d. (Set.filter
-            (\<lambda>((origin, dest), t).
-                origin = 1 \<and>
-                Label t = ''vend'' \<and>
-                length b = Arity t \<and> apply_guards (Guard t) (case_vname (\<lambda>n. input2state b 1 (I n)) (\<lambda>n. if n = 1 then Some d else None)))
-            (fset merge_1_2)) = {}"
-    apply (simp add: merge_1_2_def Set.filter_def)
-    apply safe
-    by (simp_all add: transitions)
-  show ?thesis
-    apply (case_tac "aa = ''coin'' \<and> b = [Num 50]")
-     prefer 2
-     apply (rule nondeterministic_simulates_trace.step_none)
-    using drinks_before_1_invalid
-    apply auto[1]
-    apply (rule nondeterministic_simulates_trace.step_some)
-        apply (simp add: update_before_def)
-       apply (simp add: nondeterministic_step_def possible_steps_drinks_before_coin_50)
-      apply (simp add: nondeterministic_step_def merge_1_2_update_possible_steps_coin_50 choice_coin50_coin)
-      apply auto[1]
-     apply simp
-    apply (simp add: coin50_updates coin50_updates_2)
-    by (simp add: simulation_2_1)
-qed
-
-lemma simulation_0_0: "nondeterministic_simulates_trace merge_1_2_update drinks_before 0 0 Map.empty Map.empty ((aa, b) # t) update_before"
-proof-
-  have select_updates: "length b = 1 \<Longrightarrow> (EFSM.apply_updates (Updates select) (case_vname (\<lambda>n. input2state b 1 (I n)) Map.empty) Map.empty) = <R 1 := hd b>"
-    apply (rule ext)
-    by (simp add: hd_input2state select_def)
-  have select_update_updates: "length b = 1 \<Longrightarrow> (\<lambda>x. if x = R 1 then aval (snd (R 1, V (I 1))) (case_vname (\<lambda>n. input2state b 1 (I n)) Map.empty)
-          else EFSM.apply_updates [(R 2, L (Num 0))] (case_vname (\<lambda>n. input2state b 1 (I n)) Map.empty) Map.empty x) = <R 1 := hd b, R 2 := Num 0>"
-    apply (rule ext)
-    by (simp add: hd_input2state)
-  show ?thesis
-  apply (case_tac "aa = ''select'' \<and> length b = 1")
-     apply (rule nondeterministic_simulates_trace.step_some)
-         apply (simp add: update_before_def)
-        apply (simp add: nondeterministic_step_def possible_steps_drinks_before_select)
-       apply (simp add: nondeterministic_step_def possible_steps_merge_1_2_update_select transitions)
-      apply simp
-     defer
-     apply (rule nondeterministic_simulates_trace.step_none)
-     apply (simp add: drinks_before_step_0_invalid)
-    apply (simp add: select_updates select_update_updates)
-    apply (case_tac t)
-     apply (simp add: nondeterministic_simulates_trace.base)
-    apply (case_tac a)
-    by (simp add: simulation_1_1)
-qed
-
-lemma simulation_aux: "nondeterministic_simulates_trace merge_1_2_update drinks_before 0 0 Map.empty Map.empty t update_before"
-proof (induct t)
-case Nil
-  then show ?case
-    by (simp add: nondeterministic_simulates_trace.base)
-next
-  case (Cons a t)
-  then show ?case
-    apply (case_tac a)
-    apply simp
-    by (simp add: simulation_0_0)
-qed
-
-lemma simulation: "nondeterministic_simulates merge_1_2_update drinks_before update_before"
-  apply (simp add:nondeterministic_simulates_def)
-  apply (rule allI)
-  by (simp add: simulation_aux)
-
-lemma score: "(score drinks_before naive_score) = {|(0, 2, 3), (0, 1, 3), (1, 1, 2), (0, 0, 3), (0, 0, 2), (0, 0, 1)|}"
-proof-
-  have set_filter: "(Set.filter (\<lambda>(x, y). x < y) (fset (all_pairs (S drinks_before)))) = {(2, 3), (1, 3), (1, 2), (0, 3), (0, 2), (0, 1)}"
-    apply (simp add: S_def drinks_before_def all_pairs_def Set.filter_def)
+  have ffilter: "ffilter (\<lambda>(x, y). x < y) ({|0::nat, 1, 2, 3|} |\<times>| {|0::nat, 1, 2, 3|}) = {|
+    (0, 1), (0, 2), (0, 3),
+            (1, 2), (1, 3),
+                    (2, 3)
+  |}"
+    apply (simp add: fprod_def ffilter_def fset_both_sides Abs_fset_inverse)
+    apply (simp add: Set.filter_def)
     by auto
-  have ffilter: "ffilter (\<lambda>(x, y). x < y) (all_pairs (S drinks_before)) = {|(2, 3), (1, 3), (1, 2), (0, 3), (0, 2), (0, 1)|}"
-    apply (simp add: ffilter_def set_filter)
-    by (metis finsert.rep_eq fset_inverse fset_simps(1))
-  have outgoing_transitions_2: "Set.filter (\<lambda>((origin, dest), t). origin = 2) (fset drinks_before) = {((2, 2), coin), ((2, 2), vend_fail), ((2, 3), vend_success)}"
-    apply (simp add: drinks_before_def Set.filter_def)
-    apply safe
-    by (simp_all add: transitions)
-  have abs_fset_2: "Abs_fset {((2, 2), coin), ((2, 2), vend_fail), ((2, 3), vend_success)} = {|((2, 2), coin), ((2, 2), vend_fail), ((2, 3), vend_success)|}"
-    by (metis finsert.rep_eq fset_inverse fset_simps(1))
-  have outgoing_transitions_3: "Set.filter (\<lambda>((origin, dest), t). origin = 3) (fset drinks_before) = {}"
-    apply (simp add: drinks_before_def Set.filter_def)
-    apply safe
-    by (simp_all add: transitions)
-  have outgoing_transitions_1: "Set.filter (\<lambda>((origin, dest), t). origin = 1) (fset drinks_before) = {((1, 2), coin50)}"
-    apply (simp add: drinks_before_def Set.filter_def)
-    apply safe
-    by (simp_all add: transitions)
-  have outgoing_transitions_0: "Set.filter (\<lambda>((origin, dest), t). origin = 0) (fset drinks_before) = {((0, 1), select)}"
-    apply (simp add: drinks_before_def Set.filter_def)
-    apply safe
-    by (simp_all add: transitions)
-  have naive_score_1_2: "naive_score {|coin50|} {|coin, vend_fail, vend_success|} = 1"
-    proof-
-      have abs_fset: "(Abs_fset {(coin50, coin), (coin50, vend_fail), (coin50, vend_success)}) = {|(coin50, coin), (coin50, vend_fail), (coin50, vend_success)|}"
-        by (metis finsert.rep_eq fset_inverse fset_simps(1))
-      have filter: "{(x, y). Label x = Label y \<and> Arity x = Arity y} \<inter> {(coin50, coin), (coin50, vend_fail), (coin50, vend_success)} = {(coin50, coin)}"
-        by (simp add: transitions)
-      show ?thesis
-        by (simp add: naive_score_def fprod_def abs_fset filter)
-    qed
-    have naive_score_0_2: "naive_score {|select|} {|coin, vend_fail, vend_success|} = 0"
-    proof-
-      have abs_fset: "Abs_fset {(select, coin), (select, vend_fail), (select, vend_success)} = {|(select, coin), (select, vend_fail), (select, vend_success)|}"
-        by (metis finsert.rep_eq fset_inverse fset_simps(1))
-      show ?thesis
-        apply (simp add: naive_score_def fprod_def abs_fset)
-        by (simp add: transitions)
-    qed
-    have naive_score_0_1: "naive_score {|select|} {|coin50|} = 0"
-      by (simp add: naive_score_def fprod_def transitions)
+  have score_0_1: "naive_score {|select|} {|coin50|} = 0"
+    by (simp add: naive_score_def transitions fprod_def)
+  have score_0_2: "naive_score {|select|} {|coin, vend_fail, vend_success|} = 0"
+    by (simp add: naive_score_def transitions fprod_def)
+  have score_1_2: "naive_score {|coin50|} {|coin, vend_fail, vend_success|} = 1"
+    by (simp add: naive_score_def transitions fprod_def)
+  have score: "score drinks_before naive_score = {|(0, 0, 1), (0, 0, 2), (0, 0, 3), (1, 1, 2), (0, 1, 3), (0, 2, 3)|}"
+    apply (simp add: score_def S_drinks_before ffilter)
+    apply (simp add: fimage_def outgoing_transitions_def drinks_before_def naive_score_empty)
+    by (simp add: score_0_1 score_0_2 score_1_2)
   show ?thesis
-    apply (simp add: score_def ffilter)
-    apply (simp add: outgoing_transitions_def ffilter_def)
-    apply (simp add: outgoing_transitions_2 abs_fset_2)
-    apply (simp add: outgoing_transitions_3)
-    apply (simp add: outgoing_transitions_1)
-    apply (simp add: outgoing_transitions_0)
-    by (simp add: naive_score_empty naive_score_1_2 naive_score_0_1 naive_score_0_2)
+    by (simp add: score sorted_list_of_fset_def)
 qed
 
-lemma no_choice_vend_fail_vend_success: "\<not>choice vend_fail vend_success"
-  by (simp add: choice_def transitions)
+definition merged_1_2 :: iEFSM where
+  "merged_1_2 = {|(0, (0, 1), select),
+                  (1, (1, 1), coin50),
+                  (2, (1, 1), coin),
+                  (3, (1, 1), vend_fail),
+                  (4, (1, 3), vend_success)
+                |}"
 
-lemma no_choice_coin_vend_success: "\<not>choice coin vend_success"
-  by (simp add: choice_def transitions)
+lemma merge_states_1_2: "merge_states 1 2 drinks_before = merged_1_2"
+  by (simp add: merge_states_def merge_states_aux_def drinks_before_def merged_1_2_def)
 
-lemma no_choice_coin50_vend_success: "\<not>choice coin50 vend_success"
-  by (simp add: choice_def transitions)
-
-lemma no_choice_vend_fail_coin: "\<not>choice vend_fail coin"
-  by (simp add: choice_def transitions)
-
-lemma no_choice_vend_fail_coin50: "\<not>choice vend_fail coin50"
-  by (simp add: choice_def transitions)
-
-lemma no_choice_coin_vend_fail: "\<not>choice coin vend_fail"
-  by (simp add: choice_def transitions)
-
-lemma no_choice_coin50_vend_fail: "\<not>choice coin50 vend_fail"
-  by (simp add: choice_def transitions)
-
-lemma choice_coin50_coin: "choice coin50 coin"
-  apply (simp add: choice_def transitions)
+lemma choice_coin_coin50: "choice coin coin50"
+  apply (simp add: transitions choice_def)
   by auto
 
-lemma coin50_gt_coin: "coin50 > coin"
+lemma no_choice_coin50_vend_fail: "\<not>choice coin50 vend_fail"
+  by (simp add: transitions choice_def)
+
+lemma no_choice_coin50_vend_success: "\<not>choice coin50 vend_success"
+  by (simp add: transitions choice_def)
+
+lemma no_choice_vend_fail_vend_success: "\<not>choice vend_fail vend_success"
+  by (simp add: transitions choice_def)
+
+lemma no_choice_coin_vend_fail: "\<not>choice coin vend_fail"
+  by (simp add: transitions choice_def)
+
+lemma no_choice_coin_vend_success: "\<not>choice coin vend_success"
+  by (simp add: transitions choice_def)
+
+lemmas choices = no_choice_coin_vend_success no_choice_coin_vend_fail no_choice_vend_fail_vend_success no_choice_coin50_vend_success no_choice_coin50_vend_fail choice_coin_coin50 choice_symmetry
+
+lemma coin_lt_coin50: "coin < coin50"
   by (simp add: transitions less_transition_ext_def)
 
-lemmas choices = choice_symmetry choice_coin50_coin no_choice_coin50_vend_fail no_choice_coin_vend_fail no_choice_vend_fail_vend_success no_choice_coin_vend_success no_choice_coin50_vend_success no_choice_vend_fail_coin no_choice_vend_fail_coin50
+lemmas orders = coin_lt_coin50
 
-lemma nondeterministic_pairs: "nondeterministic_pairs merge_1_2 = {|(1, (1, 1), coin, coin50)|}"
+lemma nondeterministic_pairs_merged_1_2: "nondeterministic_pairs merged_1_2 = {|(1, (1, 1), (coin, 2), coin50, 1)|}"
 proof-
-    have card1: "card {(1, coin50), (1, coin), (1, vend_fail), (3, vend_success)} = 4"
-      by (simp add: transitions)
-    have minus_1: "{|(1, coin), (1, vend_fail), (3, vend_success)|} |-| {|(1, coin50)|} = {|(1, coin), (1, vend_fail), (3, vend_success)|}"
-      by (simp add: transitions)
-    have minus_2: "{|(1, coin50), (1, coin), (1, vend_fail), (3, vend_success)|} |-| {|(1, coin)|} = {|(1, coin50), (1, vend_fail), (3, vend_success)|}"
-      apply (simp add: transitions)
-      by auto
-    have minus_3: "{|(1, coin50), (1, coin), (1, vend_fail), (3, vend_success)|} |-| {|(1, vend_fail)|} = {|(1, coin50), (1, coin), (3, vend_success)|}"
-      apply (simp add: transitions)
-      by auto
-    have minus_4: "{|(1, coin50), (1, coin), (1, vend_fail), (3, vend_success)|} |-| {|(3, vend_success)|} = {|(1, coin50), (1, coin), (1, vend_fail)|}"
-      apply (simp add: transitions)
-      by auto
-  have state_nondeterminism:  "state_nondeterminism 1 {|(1, coin50), (1, coin), (1, vend_fail), (3, vend_success)|} = {|
-   (1, (1, 3), vend_fail, vend_success),
-   (1, (1, 3), coin,    vend_success),
-   (1, (1, 3), coin50,    vend_success),
-   (1, (1, 1), vend_fail,    coin),
-   (1, (1, 1), vend_fail,    coin50),
-   (1, (1, 1), coin,    vend_fail),
-   (1, (1, 1), coin,    coin50),
-   (1, (1, 1), coin50,    vend_fail),
-   (1, (1, 1), coin50,    coin)|}"
-    apply (simp add: state_nondeterminism_def card1)
-    apply (simp only: minus_1 minus_2 minus_3 minus_4)
-    apply (simp add: fimage_def fset_both_sides Abs_fset_inverse)
-    by auto
-  show ?thesis
-    apply (simp add: nondeterministic_pairs_def)
-    apply (simp add: S_def merge_1_2_def)
-    apply (simp add: outgoing_transitions_def Set.filter_def fimage_def)
-    apply (simp add: ffilter_def state_nondeterminism)
-    apply (simp add: fset_both_sides Abs_fset_inverse Set.filter_def)
-    apply safe
-                        apply (simp_all add: choices)
-    using coin50_gt_coin choice_coin50_coin choice_symmetry by auto
-qed
-
-lemma coin_doesnt_exit_1_drinks_before: "\<not>exits_state drinks_before coin 1"
-proof-
-  have set_filter: "Set.filter (\<lambda>((from', to), t'). from' = 1 \<and> t' = coin) (fset drinks_before) = {}"
-    apply (simp add: drinks_before_def Set.filter_def)
-    apply safe
-    by (simp_all add: transitions)
-  show ?thesis
-    by (simp add: exits_state_def ffilter_def set_filter)
-qed
-
-lemma coin50_exits_1_drinks_before: "exits_state drinks_before coin50 1"
-proof-
-  have set_filter: "Set.filter (\<lambda>((from', to), t'). from' = 1 \<and> t' = coin50) (fset drinks_before) = {((1, 2), coin50)}"
-    apply (simp add: drinks_before_def Set.filter_def)
-    apply safe
-    by (simp_all add: transitions)
-  show ?thesis
-    by (simp add: exits_state_def ffilter_def set_filter)
-qed
-
-lemma select_first: "\<not> (aa = ''select'' \<and> length b = 1) \<Longrightarrow> \<not>gets_us_to 1 merge_1_2_update 0 Map.empty ((aa, b) # p)"
-      proof-
-        assume premise: "\<not> (aa = ''select'' \<and> length b = 1)"
-        have set_filter: "(Set.filter
-                (\<lambda>((origin, dest), t).
-                    origin = 0 \<and>
-                    Label t = aa \<and> length b = Arity t \<and> apply_guards (Guard t) (case_vname (\<lambda>n. input2state b 1 (I n)) Map.empty))
-                (fset merge_1_2_update)) = {}"
-          using premise
-          apply (simp add: Set.filter_def merge_1_2_update_def)
-          apply safe
-          by (simp_all add: transitions)
-      show ?thesis
-        apply safe
-        apply (rule gets_us_to.cases)
-           apply simp
-          apply simp
-         apply clarify
-         apply (simp add: step_def possible_steps_def ffilter_def set_filter)
-        apply clarify
-        by (simp add: step_def possible_steps_def ffilter_def set_filter)
-    qed
-
-lemma no_subsumption_empty: "\<not> subsumes \<lbrakk>\<rbrakk> coin coin50"
-proof-
-  have violation: "(\<exists>i r. satisfies_context r \<lbrakk>\<rbrakk> \<and>
-           apply_guards (Guard coin50) (case_vname (\<lambda>n. input2state i 1 (I n)) (\<lambda>n. r (R n))) \<and>
-           apply_outputs (Outputs coin50) (case_vname (\<lambda>n. input2state i 1 (I n)) (\<lambda>n. r (R n))) \<noteq>
-           apply_outputs (Outputs coin) (case_vname (\<lambda>n. input2state i 1 (I n)) (\<lambda>n. r (R n))))"
-    apply (rule_tac x="[Num 50]" in exI)
-    apply (rule_tac x="<>" in exI)
+  have minus_1: "{(1, coin50, 1), (1, coin, 2), (1, vend_fail, 3), (3, vend_success, 4)} - {(1, coin, 2)} = {(1, coin50, 1), (1, vend_fail, 3), (3, vend_success, 4)}"
     apply (simp add: transitions)
-    apply (simp add: satisfies_context_def datastate2context_def consistent_def)
-    apply (rule_tac x="<>" in exI)
-    apply safe
-    apply (case_tac r)
-       apply simp
-      apply simp
-      apply (case_tac x2)
-       apply simp
-      apply simp
-     apply simp
-    by simp
-  show ?thesis
-    by (simp add: subsumes_def violation)
-qed
-
-lemma satisfies_must_have_r2_0: "satisfies_context d \<lbrakk>V (R 1) \<mapsto> cexp.Bc True, V (R 2) \<mapsto> cexp.Eq (Num 0)\<rbrakk> \<Longrightarrow> d (R 2) = Some (Num 0)"
-proof-
-  have contrapositive: "\<not> d (R 2) = Some (Num 0) \<Longrightarrow> \<not>satisfies_context d \<lbrakk>V (R 1) \<mapsto> cexp.Bc True, V (R 2) \<mapsto> cexp.Eq (Num 0)\<rbrakk>"
-    apply (simp add: satisfies_context_def datastate2context_def consistent_def)
-    apply (rule allI)
-    apply (rule_tac x="V (R 2)" in exI)
-    apply simp
-    apply (case_tac "d (R 2)")
-     apply simp
-    by simp
-  show "satisfies_context d \<lbrakk>V (R 1) \<mapsto> cexp.Bc True, V (R 2) \<mapsto> cexp.Eq (Num 0)\<rbrakk> \<Longrightarrow> d (R 2) = Some (Num 0)"
-    using contrapositive
     by auto
-qed 
-
-lemma consistent_medial_coin: "consistent \<lbrakk>V (R 1) \<mapsto> cexp.Bc True, V (R 2) \<mapsto> cexp.Eq (Num 0)\<rbrakk>"
-    apply (simp add: consistent_def)
-    apply (rule_tac x="<R 1 := Str ''coke'', R 2 := Num 0, I 1 := Num 50>" in exI)
-    apply (rule allI)
-    by (simp add: consistent_empty_4)
-
-lemma coin_posterior: "posterior \<lbrakk>V (R 1) \<mapsto> cexp.Bc True, V (R 2) \<mapsto> cexp.Eq (Num 0)\<rbrakk> coin = 
-                       \<lbrakk>V (R 1) \<mapsto> cexp.Bc True, V (R 2) \<mapsto> cexp.Bc True\<rbrakk>"
-  apply (simp add: posterior_def Let_def transitions satisfiable_def remove_input_constraints_def)
-  apply standard
-  apply clarify
-   apply (rule ext)
-   apply simp
-  by (simp add: consistent_medial_coin)
-
-lemma coin_subsumes_coin50: "subsumes \<lbrakk>V (R 1) \<mapsto> cexp.Bc True, V (R 2) \<mapsto> cexp.Eq (Num 0)\<rbrakk> coin coin50"
-proof-
-  have medial_coin50: "medial \<lbrakk>V (R 1) \<mapsto> cexp.Bc True, V (R 2) \<mapsto> cexp.Eq (Num 0)\<rbrakk> (Guard coin50) =
-        \<lbrakk>V (R 1) \<mapsto> cexp.Bc True, V (R 2) \<mapsto> cexp.Eq (Num 0), V (I 1) \<mapsto> Eq (Num 50)\<rbrakk>"
-    apply (rule ext)
-    by (simp add: transitions)
-  have consistent_medial_coin50: "consistent \<lbrakk>V (R 1) \<mapsto> cexp.Bc True, V (R 2) \<mapsto> cexp.Eq (Num 0), V (I 1) \<mapsto> cexp.Eq (Num 50)\<rbrakk>"
-    apply (simp add: consistent_def)
-    apply (rule_tac x="<R 1 := Str ''coke'', R 2 := Num 0, I 1 := Num 50>" in exI)
-    apply (rule allI)
-    by (simp add: consistent_empty_4)
-  have apply_coin50_updates: "(remove_input_constraints
-              (Contexts.apply_updates \<lbrakk>V (R 1) \<mapsto> cexp.Bc True, V (R 2) \<mapsto> cexp.Eq (Num 0), V (I 1) \<mapsto> cexp.Eq (Num 50)\<rbrakk>
-                \<lbrakk>V (R 1) \<mapsto> cexp.Bc True, V (R 2) \<mapsto> cexp.Eq (Num 0)\<rbrakk> (Updates coin50))) = \<lbrakk>V (R 1) \<mapsto> cexp.Bc True, V (R 2) \<mapsto> cexp.Eq (Num 50)\<rbrakk>"
-    apply (rule ext)
-    by (simp add: coin50_def remove_input_constraints_def)
-  have apply_coin_updates: "remove_input_constraints
-                  (Contexts.apply_updates \<lbrakk>V (R 1) \<mapsto> cexp.Bc True, V (R 2) \<mapsto> cexp.Eq (Num 0), V (I 1) \<mapsto> cexp.Eq (Num 50)\<rbrakk>
-                    \<lbrakk>V (R 1) \<mapsto> cexp.Bc True, V (R 2) \<mapsto> cexp.Eq (Num 0), V (I 1) \<mapsto> cexp.Eq (Num 50)\<rbrakk> (Updates coin)) = \<lbrakk>V (R 1) \<mapsto> cexp.Bc True, V (R 2) \<mapsto> cexp.Eq (Num 50)\<rbrakk>"
-    apply (rule ext)
-    apply (simp add: coin_def remove_input_constraints_def valid_def satisfiable_def)
-    by auto
-  show ?thesis
-    unfolding subsumes_def
-    apply standard
-     apply (simp add: transitions)
-    apply standard
-     apply (simp add: transitions)
-    apply standard
-     apply (simp add: transitions)
-    apply standard
-     apply (simp add: transitions)
-     apply clarify
-     apply (case_tac "cval (\<lbrakk>\<rbrakk> r) i")
-      apply simp
-     apply simp
-    apply standard
-     apply (simp add: transitions)
-     apply clarify
-     apply (case_tac "value_plus (r (R 2)) (Some (Num 50))")
-      apply simp
-    using satisfies_must_have_r2_0
-      apply fastforce
-     apply simp
-    using satisfies_must_have_r2_0
-     apply fastforce
-    apply standard
-     apply (simp add: medial_coin50)
-     apply clarify
-     apply (simp add: posterior_def Let_def guard_coin medial_coin50)
-     apply (simp add: consistent_medial_coin50)
-     apply (simp add: apply_coin50_updates apply_coin_updates)
-    apply (simp add: consistent_def)
-    apply safe
-    apply (rule_tac x=s in exI)
-    apply (simp add: posterior_def Let_def)
-    apply (simp add: medial_coin50 consistent_medial_coin50)
-    apply (simp add: apply_coin50_updates)
-    apply (simp add: guard_coin consistent_medial_coin)
-    apply (simp add: coin_def remove_input_constraints_def satisfiable_def)
-    by (simp add: consistent_empty_4)
-qed
-
-lemma step_vend_fail: "step merge_1_2_update 1 <R 1 := hd b, R 2 := Num 0> ''vend'' [] = Some (vend_fail, 1, [], <R 1 := hd b, R 2 := Num 0>)"
-proof-
-  have set_filter: "(Set.filter
-          (\<lambda>((origin, dest), t).
-              origin = 1 \<and>
-              Label t = ''vend'' \<and>
-              Arity t = 0 \<and> apply_guards (Guard t) (case_vname Map.empty (\<lambda>n. if n = 2 then Some (Num 0) else <R 1 := hd b> (R n))))
-          (fset merge_1_2_update)) = {((1, 1), vend_fail)}"
-    apply (simp add: merge_1_2_update_def Set.filter_def)
-    apply safe
-    by (simp_all add: transitions)
-  show ?thesis
-    apply (simp add: step_def possible_steps_def ffilter_def set_filter)
-    apply (simp add: step_def possible_steps_def ffilter_def set_filter)
-    by (simp add: vend_fail_def)
-qed
-
-lemma posterior_vend_fail: "posterior \<lbrakk>V (R 1) \<mapsto> cexp.Bc True, V (R 2) \<mapsto> cexp.Eq (Num 0)\<rbrakk> vend_fail =
-       \<lbrakk>V (R 1) \<mapsto> cexp.Bc True, V (R 2) \<mapsto> cexp.Eq (Num 0)\<rbrakk>"
-proof-
-  have medial: "medial \<lbrakk>V (R 1) \<mapsto> cexp.Bc True, V (R 2) \<mapsto> cexp.Eq (Num 0)\<rbrakk> (Guard vend_fail) =
-        \<lbrakk>V (R 1) \<mapsto> cexp.Bc True, V (R 2) \<mapsto> And (cexp.Eq (Num 0)) (cexp.Lt (Num 100))\<rbrakk>"
-    apply (rule ext)
-    by (simp add: vend_fail_def)
-  have consistent: "consistent \<lbrakk>V (R 1) \<mapsto> cexp.Bc True, V (R 2) \<mapsto> And (cexp.Eq (Num 0)) (cexp.Lt (Num 100))\<rbrakk>"
-    apply (simp add: consistent_def)
-    apply (rule_tac x="<R 1 := Num 5, R 2 := Num 0>" in exI)
-    apply clarify
-    by (simp add: consistent_empty_4)
-  show ?thesis
-    unfolding posterior_def Let_def
-    apply (simp add: medial consistent remove_input_constraints_def)
-    apply (rule ext)
-    by (simp add: vend_fail_def)
-qed
-
-lemma merge_1_2_step_0_invalid: "\<not> (aa = ''select'' \<and> length b = 1) \<Longrightarrow> nondeterministic_step merge_1_2 0 Map.empty aa b = None"
-proof-
-  assume premise: "\<not> (aa = ''select'' \<and> length b = 1)"
-  have set_filter: "Set.filter
-           (\<lambda>((origin, dest), t).
-               origin = 0 \<and> Label t = aa \<and> length b = Arity t \<and> apply_guards (Guard t) (case_vname (\<lambda>n. input2state b 1 (I n)) Map.empty))
-           (fset merge_1_2) = {}"
-    using premise
-    apply (simp add: merge_1_2_def Set.filter_def)
-    apply safe
-    by (simp_all add: transitions)
-  show ?thesis
-    by (simp add: nondeterministic_step_def possible_steps_def ffilter_def set_filter)
-qed
-
-lemma nondeterministic_step_merge_1_2_1_invalid: "aa \<noteq> ''coin'' \<Longrightarrow> nondeterministic_step merge_1_2 1 <R 1 := d> aa b = None"
-proof-
-  assume premise: "aa \<noteq> ''coin''"
-  have set_filter: "Set.filter
-           (\<lambda>((origin, dest), t).
-               origin = 1 \<and>
-               Label t = aa \<and>
-               length b = Arity t \<and> apply_guards (Guard t) (case_vname (\<lambda>n. input2state b 1 (I n)) (\<lambda>n. if n = 1 then Some d else None)))
-           (fset merge_1_2) = {}"
-    using premise
-    apply (simp add: Set.filter_def merge_1_2_def)
-    apply safe
-    by (simp_all add: transitions)
-  show ?thesis
-    by (simp add: nondeterministic_step_def possible_steps_def ffilter_def set_filter)
-qed
-
-lemma nondeterministic_step_merge_1_2_1_invalid_coin: "aa = ''coin'' \<Longrightarrow> length b \<noteq> 1 \<Longrightarrow> nondeterministic_step merge_1_2 1 <R 1 := d> aa b = None"
-proof-
-  assume premise1: "aa = ''coin''"
-  assume premise2: "length b \<noteq> 1"
-  have set_filter: "Set.filter
-           (\<lambda>((origin, dest), t).
-               origin = 1 \<and>
-               Label t = aa \<and>
-               length b = Arity t \<and> apply_guards (Guard t) (case_vname (\<lambda>n. input2state b 1 (I n)) (\<lambda>n. if n = 1 then Some d else None)))
-           (fset merge_1_2) = {}"
-    using premise1 premise2
-    apply (simp add: merge_1_2_def Set.filter_def)
-    apply safe
-    by (simp_all add: transitions)
-  show ?thesis
-    by (simp add: nondeterministic_step_def possible_steps_def ffilter_def set_filter)
-qed
-
-lemma nondeterministic_step_merge_1_2_1_silly_coin: "length b = 1 \<Longrightarrow> b \<noteq> [Num 50] \<Longrightarrow> nondeterministic_step merge_1_2 1 <R 1 := d> ''coin'' b = Some (coin, 1, [None], <R 1 := d>)"
-proof-
-  assume premise1: "length b = 1"
-  assume premise2: "b \<noteq> [Num 50]"
-  have set_filter: "Set.filter
-            (\<lambda>((origin, dest), t).
-                origin = 1 \<and>
-                Label t = ''coin'' \<and>
-                length b = Arity t \<and> apply_guards (Guard t) (case_vname (\<lambda>n. input2state b 1 (I n)) (\<lambda>n. if n = 1 then Some d else None)))
-            (fset merge_1_2) = {((1, 1), coin)}"
-    using premise1 premise2
-    apply (simp add: Set.filter_def merge_1_2_def)
-    apply safe
-           apply (simp_all add: transitions hd_input2state)
-    by (metis One_nat_def length_0_conv length_Suc_conv list.sel(1))
-  show ?thesis
-    apply (simp add: nondeterministic_step_def possible_steps_def ffilter_def set_filter)
-    apply (simp add: set_filter)
+  have minus_2: "{(1, coin50, 1), (1, coin, 2), (1, vend_fail, 3), (3, vend_success, 4)} - {(1, vend_fail, 3)} = {(1, coin50, 1), (1, coin, 2), (3, vend_success, 4)}"
     apply (simp add: transitions)
-    apply (rule ext)
-    by simp
-qed
-
-lemma easy_merge_some: "easy_merge drinks_before merge_1_2_update 2 1 1 1 1 coin coin50 (\<lambda>a b c d. Map.empty) = Some drinks_after"
-  apply (simp add: easy_merge_def)
-  oops
-
-lemma score_2: "sorted_list_of_fset (score drinks_after naive_score) = [(0, 0, 1), (0, 0, 3), (0, 1, 3)]"
-proof-
-  have set_filter: "Set.filter (\<lambda>(x, y). x < y) (fset (all_pairs (S drinks_after))) = {(1, 3), (0, 3), (0, 1)}"
-    apply (simp add: Set.filter_def all_pairs_def S_def drinks_after_def)
     by auto
-  have abs_fset: "Abs_fset {(1, 3), (0, 3), (0, 1)} = {|(1, 3), (0, 3), (0, 1)|}"
-    by (metis finsert.rep_eq fset_inverse fset_simps(1))
-  have outgoing_transitions_1: "Set.filter (\<lambda>((origin, dest), t). origin = 1) (fset drinks_after) = {((1, 1), coin), ((1, 1), vend_fail), ((1, 3), vend_success)}"
-    apply (simp add: drinks_after_def Set.filter_def)
-    apply safe
-    by (simp_all add: transitions)
-  have abs_fset_1: "Abs_fset {((1, 1), coin), ((1, 1), vend_fail), ((1, 3), vend_success)} =
-                            {|((1, 1), coin), ((1, 1), vend_fail), ((1, 3), vend_success)|}"
-    by (metis finsert.rep_eq fset_inverse fset_simps(1))
-  have outgoing_transitions_3: "Set.filter (\<lambda>((origin, dest), t). origin = 3) (fset drinks_after) = {}"
-    apply (simp add: drinks_after_def Set.filter_def)
-    apply safe
-    by (simp_all add: transitions)
-  have outgoing_transitions_0: "Set.filter (\<lambda>((origin, dest), t). origin = 0) (fset drinks_after) = {((0, 1), select_update)}"
-    apply (simp add: drinks_after_def Set.filter_def)
-    apply safe
-    by (simp_all add: transitions)
-  have score_0_1: "naive_score {|select_update|} {|coin, vend_fail, vend_success|} = 0"
-  proof-
-    have abs_fset: "Abs_fset {(select_update, coin), (select_update, vend_fail), (select_update, vend_success)} = 
-                  {|(select_update, coin), (select_update, vend_fail), (select_update, vend_success)|}"
-      by (metis finsert.rep_eq fset_inverse fset_simps(1))
-    show ?thesis
-      apply (simp add: naive_score_def fprod_def abs_fset)
-      by (simp add: transitions)
-  qed
+  have minus_3: "{(1, coin50, 1), (1, coin, 2), (1, vend_fail, 3), (3, vend_success, 4)} - {(3, vend_success, 4)} = {(1, coin50, 1), (1, coin, 2), (1, vend_fail, 3)}"
+    apply (simp add: transitions)
+    by auto
+  have state_nondeterminism_1: "state_nondeterminism 1 {|(1, coin50, 1), (1, coin, 2), (1, vend_fail, 3), (3, vend_success, 4)|} = {|
+      (1, (1, 1), (coin50, 1), coin, 2),
+      (1, (1, 1), (coin50, 1), vend_fail, 3),
+      (1, (1, 3), (coin50, 1), vend_success, 4),
+      (1, (1, 3), (vend_fail, 3), vend_success, 4),
+      (1, (1, 1), (vend_fail, 3), coin50, 1),
+      (1, (1, 1), (vend_fail, 3), coin, 2),
+      (1, (1, 1), (coin, 2), coin50, 1),
+      (1, (1, 1), (coin, 2), vend_fail, 3),
+      (1, (1, 3), (coin, 2), vend_success, 4)
+    |}"
+    apply (simp add: state_nondeterminism_def fimage_def fset_both_sides Abs_fset_inverse)
+    apply (simp add: minus_1 minus_2 minus_3)
+    by auto
   show ?thesis
-    apply (simp add: score_def ffilter_def set_filter abs_fset)
-    apply (simp add: outgoing_transitions_def ffilter_def)
-    apply (simp add: outgoing_transitions_1 abs_fset_1)
-    apply (simp add: outgoing_transitions_3)
-    apply (simp add: outgoing_transitions_0)
-    apply (simp add: naive_score_empty score_0_1)
-    by (simp add: sorted_list_of_fset_def)
+    apply (simp add: nondeterministic_pairs_def S_def merged_1_2_def)
+    apply (simp add: outgoing_transitions_def fimage_def state_nondeterminism_1)
+    apply (simp add: ffilter_def fset_both_sides Abs_fset_inverse Set.filter_def)
+    apply safe
+    using choices orders by auto
 qed
 
-lemma step_drinks_before_select: "length ba = 1 \<Longrightarrow> step drinks_before 0 Map.empty ''select'' ba = Some (select, 1, [], <R 1 := hd ba>)"
+lemma step_drinks_before_select: "length ba = 1 \<Longrightarrow> step (tm drinks_before) 0 Map.empty ''select'' ba = Some (select, 1, [], <R 1 := hd ba>)"
 proof-
   assume premise: "length ba = 1"
+  have possible_steps: "possible_steps (tm drinks_before) 0 Map.empty ''select'' ba = {|(1, select)|}"
+    apply (simp add: possible_steps_def ffilter_def fimage_def fset_both_sides Abs_fset_inverse)
+    apply (simp add: tm_def drinks_before_def Set.filter_def)
+    apply safe
+    using premise
+            apply (simp_all add: transitions)
+    by force
   show ?thesis
-     apply (simp add: premise step_def possible_steps_drinks_before_select)
+    apply (simp add: step_def possible_steps)
     apply (simp add: select_def)
     apply (rule ext)
     by (simp add: hd_input2state premise)
 qed
 
-lemma no_direct_subsumption_coin_coin50: "\<not> directly_subsumes drinks_before merge_1_2 1 coin coin50"
+lemma possible_steps_merge_1_2_select: "length b = 1 \<Longrightarrow> possible_steps (tm merged_1_2) 0 r ''select'' b = {|(1, select)|}"
+  apply (simp add: possible_steps_def ffilter_def fimage_def fset_both_sides Abs_fset_inverse)
+  apply (simp add: tm_def merged_1_2_def Set.filter_def)
+  apply safe
+       apply (simp_all add: transitions)
+  by force
+
+lemma no_direct_subsumption_coin_coin50: "\<not> directly_subsumes (tm drinks_before) (tm merged_1_2) 1 coin coin50"
 proof-
   have subsumption_violation: "(\<exists>i r. satisfies_context r \<lbrakk>V (R 1) \<mapsto> cexp.Bc True\<rbrakk> \<and>
            apply_guards (Guard coin50) (case_vname (\<lambda>n. input2state i 1 (I n)) (\<lambda>n. r (R n))) \<and>
@@ -1025,56 +254,42 @@ proof-
      apply (rule accepts.base)
     apply standard
      apply (rule gets_us_to.step_some)
-      apply (simp add: step_def possible_steps_drinks_before_select)
+      apply (simp add: step_drinks_before_select)
      apply (simp add: gets_us_to.base)
     apply (simp add: anterior_context_def step_def possible_steps_merge_1_2_select select_posterior)
     by (simp add: subsumes_def subsumption_violation)
 qed
 
-lemma possible_steps_merge_1_2_coin50: "possible_steps merge_1_2 1 r ''coin'' [Num 50] = {|(1, coin), (1, coin50)|}"
+lemma step_drinks_before_coin_50: "step (tm drinks_before) 1 <R 1 := d> ''coin'' [Num 50] = Some (coin50, 2, [Some (Num 50)], <R 1 := d, R 2 := Num 50>)"
 proof-
-  have set_filter: "Set.filter
-       (\<lambda>((origin, dest), t).
-           origin = 1 \<and>
-           Label t = ''coin'' \<and> Suc 0 = Arity t \<and> apply_guards (Guard t) (case_vname (\<lambda>n. input2state [Num 50] 1 (I n)) (\<lambda>n. r (R n))))
-       (fset merge_1_2) = {((1, 1), coin), ((1, 1), coin50)}"
-    apply (simp add: Set.filter_def merge_1_2_def)
+  have possible_steps: "possible_steps (tm drinks_before) 1 <R 1 := d> ''coin'' [Num 50] = {|(2, coin50)|}"
+    apply (simp add: possible_steps_def ffilter_def fimage_def fset_both_sides Abs_fset_inverse)
+    apply (simp add: Set.filter_def tm_def drinks_before_def)
     apply safe
-    by (simp_all add: transitions)
-  have abs_fset: "Abs_fset {((1, 1), coin), ((1, 1), coin50)} = {|((1, 1), coin), ((1, 1), coin50)|}"
-    by (metis finsert.rep_eq fset_inverse fset_simps(1))
+          apply (simp_all add: transitions)
+    by force
   show ?thesis
-    by (simp add: possible_steps_def ffilter_def set_filter abs_fset)
-qed
-
-lemma step_drinks_before_coin_50: "step drinks_before 1 <R 1 := d> ''coin'' [Num 50] = Some (coin50, 2, [Some (Num 50)], <R 1 := d, R 2 := Num 50>)"
-proof-
-  have set_filter: "Set.filter
-          (\<lambda>((origin, dest), t).
-              origin = 1 \<and>
-              Label t = ''coin'' \<and>
-              Suc 0 = Arity t \<and>
-              apply_guards (Guard t)
-               (case_vname (\<lambda>n. if n = 1 then Some (Num 50) else input2state [] (1 + 1) (I n)) (\<lambda>n. if n = 1 then Some d else None)))
-          (fset drinks_before) = {((1, 2), coin50)}"
-    apply (simp add: Set.filter_def drinks_before_def)
-    apply safe
-    by (simp_all add: transitions)
-  show ?thesis
-    apply (simp add: step_def possible_steps_def ffilter_def set_filter)
-    apply (simp add: set_filter)
-    apply (simp add: transitions)
+    apply (simp add: step_def possible_steps)
+    apply (simp add: coin50_def)
     apply (rule ext)
     by simp
 qed
 
-lemma no_direct_subsumption_coin50_coin: "\<not> directly_subsumes drinks_before merge_1_2 2 coin50 coin"
+lemma possible_steps_merge_1_2_coin50: "possible_steps (tm merged_1_2) 1 r ''coin'' [Num 50] = {|(1, coin), (1, coin50)|}"
+  apply (simp add: possible_steps_def ffilter_def fimage_def fset_both_sides Abs_fset_inverse)
+  apply (simp add: Set.filter_def tm_def merged_1_2_def)
+  apply safe
+         apply (simp_all add: transitions)
+   apply force
+  by force
+
+lemma no_direct_subsumption_coin50_coin: "\<not> directly_subsumes (tm drinks_before) (tm merged_1_2) 2 coin50 coin"
 proof-
   have subsumption_violation: "(\<exists>i r. satisfies_context r \<lbrakk>V (R 1) \<mapsto> cexp.Bc True\<rbrakk> \<and>
            apply_guards (Guard coin) (case_vname (\<lambda>n. input2state i 1 (I n)) (\<lambda>n. r (R n))) \<and>
            apply_outputs (Outputs coin) (case_vname (\<lambda>n. input2state i 1 (I n)) (\<lambda>n. r (R n))) \<noteq>
            apply_outputs (Outputs coin50) (case_vname (\<lambda>n. input2state i 1 (I n)) (\<lambda>n. r (R n))))"
-apply (rule_tac x="[Num 50]" in exI)
+    apply (rule_tac x="[Num 50]" in exI)
     apply (rule_tac x="<R 1 := Str ''coke''>" in exI)
     apply standard
      defer
@@ -1100,9 +315,9 @@ apply (rule_tac x="[Num 50]" in exI)
     apply (rule accepts.base)
     apply standard
      apply (rule gets_us_to.step_some)
-      apply (simp add: step_def possible_steps_drinks_before_select)
+      apply (simp add: step_drinks_before_select)
      apply (rule gets_us_to.step_some)
-      apply (simp add: step_def possible_steps_drinks_before_coin_50)
+      apply (simp add: step_drinks_before_coin_50)
      apply (simp add: gets_us_to.base)
     apply (simp add: anterior_context_def step_def possible_steps_merge_1_2_select select_posterior)
     apply (simp add: possible_steps_merge_1_2_coin50 fis_singleton_def is_singleton_def)
@@ -1111,328 +326,85 @@ apply (rule_tac x="[Num 50]" in exI)
     by (simp add: subsumes_def subsumption_violation)
 qed
 
-lemma easy_merge_none:  "easy_merge drinks_before merge_1_2 2 1 1 1 1 coin coin50 (\<lambda>a b c d. Map.empty) = None"
-  by (simp add: easy_merge_def no_direct_subsumption_coin_coin50 no_direct_subsumption_coin50_coin)
-
-lemma regsimp1: "(\<lambda>a. if a = R 1 then Some d else None) = <R 1 := d>"
-  by auto
-
-lemma contextsimp1: "(\<lambda>a. if a = V (R 2) then cexp.Eq (Num 0) else if a = V (R 1) then cexp.Bc True else \<lbrakk>\<rbrakk> a) = 
-                     \<lbrakk>V (R 1) \<mapsto> cexp.Bc True, V (R 2) \<mapsto> cexp.Eq (Num 0)\<rbrakk>"
-  by auto
-
-lemma regsimp2: "(\<lambda>a. if a = R 2 then Some (Num n) else if a = R 1 then Some d else None) = <R 1 := d, R 2 := Num n>"
-  by auto
-
-lemma invalid_r2_vend: "\<nexists>n. ra (R 2) = Some (Num n) \<Longrightarrow> step drinks_before 2 ra ''vend'' [] = None"
+lemma simulation_0_0: "nondeterministic_simulates_trace (tm merge_1_2_update) (tm drinks_before) 0 0 Map.empty Map.empty ((aa, b) # t) update_before"
 proof-
-  assume premise: "\<nexists>n. ra (R 2) = Some (Num n)"
-  have set_filter: "(Set.filter
-         (\<lambda>((origin, dest), t). origin = 2 \<and> Label t = ''vend'' \<and> Arity t = 0 \<and> apply_guards (Guard t) (case_vname Map.empty (\<lambda>n. ra (R n))))
-         (fset drinks_before)) = {}"
-    using premise
-    apply (simp add: Set.filter_def drinks_before_def)
-    apply safe
-      apply (simp add: transitions)
-    apply (simp add: transitions)
-     apply (metis MaybeBoolInt.elims option.simps(3))
-    apply (simp add: transitions)
-    apply (case_tac "MaybeBoolInt (\<lambda>x y. y < x) (Some (Num 100)) (ra (R 2))")
-     apply simp
-    apply simp
-    by (metis MaybeBoolInt.elims option.simps(3))
-  show ?thesis
-    by (simp add: step_def possible_steps_def ffilter_def set_filter)
-qed
-
-lemma step_drinks_before_vend_fail: "ra (R 2) = Some (Num x1) \<Longrightarrow> x1 < 100 \<Longrightarrow> step drinks_before 2 ra ''vend'' [] = Some (vend_fail, 2, [], ra)"
-proof-
-  assume premise1: "ra (R 2) = Some (Num x1)"
-  assume premise2: "x1 < 100"
-  have set_filter: "Set.filter
-          (\<lambda>((origin, dest), t).
-              origin = 2 \<and> Label t = ''vend'' \<and> Arity t = 0 \<and> apply_guards (Guard t) (case_vname Map.empty (\<lambda>n. ra (R n))))
-          (fset drinks_before) = {((2, 2), vend_fail)}"
-    using premise1 premise2
-    apply (simp add: Set.filter_def drinks_before_def)
-    apply safe
-    by (simp_all add: transitions)
-  show ?thesis
-    apply (simp add: step_def possible_steps_def ffilter_def set_filter)
-    apply (simp add: set_filter)
-    by (simp add: transitions)
-qed
-
-lemma step_drinks_before_3_none: "step drinks_before 3 r' a b = None"
-proof-
-  have set_filter: "Set.filter
-         (\<lambda>((origin, dest), t).
-             origin = 3 \<and> Label t = a \<and> length b = Arity t \<and> apply_guards (Guard t) (case_vname (\<lambda>n. input2state b 1 (I n)) (\<lambda>n. r' (R n))))
-         (fset drinks_before) = {}"
-    by (simp add: Set.filter_def drinks_before_def)
-  show ?thesis
-    by (simp add: step_def possible_steps_def ffilter_def set_filter)
-qed
-
-lemma no_route_from_3_to_anywhere: "s \<noteq> 3 \<Longrightarrow> \<not>gets_us_to s drinks_before 3 r' p"
-  apply safe
-  apply (rule gets_us_to.cases)
-     apply simp
-    apply simp
-   apply (simp add: step_drinks_before_3_none)
-  by simp
-
-lemma no_route_from_2_to_1: "\<forall>r. \<not>gets_us_to 1 drinks_before 2 r p"
-proof(induct p)
-  case Nil
-  then show ?case
-    by (simp add: no_further_steps)
-next
-  case (Cons a p)
-  then show ?case
-    apply clarify
-    apply (rule gets_us_to.cases)
-       apply simp
-      apply simp
-     defer
-     apply simp
-    apply clarify
-    apply simp
-    apply (case_tac "aa = ''coin'' \<and> length b = 1")
-     apply (simp add: step_def possible_steps_drinks_before_coin)
-    apply (case_tac "aa = ''vend'' \<and> b = []")
-    defer
-    apply (simp add: nondeterministic_step_drinks_before_invalid_step_2 nondeterministic_step_none)
-     apply clarify
-     apply simp
-     apply (case_tac "ra (R 2)")
-      apply (simp add: invalid_r2_vend)
-     apply (case_tac aa)
-      defer
-     apply (simp add: invalid_r2_vend)
-    apply clarify
-    apply simp
-    apply (case_tac "x1 < 100")
-     apply (simp add: step_drinks_before_vend_fail)
-    apply (simp add: step_def drinks_before_vend_success)
-    apply (simp add: vend_success_def)
-    apply clarify
-    by (simp add: no_route_from_3_to_anywhere)
-qed
-
-lemma drinks_before_1_step_invalid: "(aa, ba) \<noteq> (''coin'', [Num 50]) \<Longrightarrow> step drinks_before 1 r aa ba = None"
-proof-
-  assume premise: "(aa, ba) \<noteq> (''coin'', [Num 50])"
-  have set_filter: "Set.filter
-         (\<lambda>((origin, dest), t).
-             origin = 1 \<and>
-             Label t = aa \<and> length ba = Arity t \<and> apply_guards (Guard t) (case_vname (\<lambda>n. input2state ba 1 (I n)) (\<lambda>n. r (R n))))
-         (fset drinks_before) = {}"
-    using premise
-    apply (simp add: Set.filter_def drinks_before_def)
-    apply safe
-     apply (simp_all add: transitions)
-    by (metis One_nat_def hd_input2state le_numeral_extra(4) length_0_conv length_Suc_conv list.sel(1) option.inject)
-  show ?thesis
-    by (simp add: step_def possible_steps_def ffilter_def set_filter)
-qed
-
-lemma stop_at_1: "step drinks_before 1 <R 1 := d> aa ba = Some (uw, s', ux, r') \<Longrightarrow> \<not>gets_us_to 1 drinks_before 1 <R 1 := d> ((aa, ba) # p)"
-  apply safe
-  apply (rule gets_us_to.cases)
-     apply simp
-    apply simp
-  apply (case_tac "(aa, ba) = (''coin'', [Num 50])")
-   apply (simp add: step_drinks_before_coin_50)
-    apply clarify
-    apply simp
-    apply clarify
-    apply simp
-   apply (simp add: step_drinks_before_coin_50)
-    apply clarify
-    apply (simp add: no_route_from_2_to_1)
-   apply (simp add: drinks_before_1_step_invalid)
-   apply clarify
-  by simp
-
-lemma drinks_before_1_must_be_coin_50: "fis_singleton (possible_steps drinks_before 1 <R 1 := d> aa ba) \<Longrightarrow> (aa = ''coin'' \<and> ba = [Num 50])"
-proof-
-  assume premise: "fis_singleton (possible_steps drinks_before 1 <R 1 := d> aa ba)"
-  have set_filter: "\<not> (aa = ''coin'' \<and> ba = [Num 50]) \<Longrightarrow> Set.filter
-         (\<lambda>((origin, dest), t).
-             origin = 1 \<and>
-             Label t = aa \<and>
-             length ba = Arity t \<and> apply_guards (Guard t) (case_vname (\<lambda>n. input2state ba 1 (I n)) (\<lambda>n. if n = 1 then Some d else None)))
-         (fset drinks_before) = {}"
-    apply (simp add: Set.filter_def drinks_before_def)
-    apply (simp add: transitions)
-    by (metis One_nat_def hd_input2state le_numeral_extra(4) length_0_conv length_Suc_conv list.sel(1) option.inject)
-  show ?thesis
-    using premise
-    apply (case_tac "aa = ''coin'' \<and> ba = [Num 50]")
-     apply simp
-    by (simp add: possible_steps_def ffilter_def set_filter)
-qed
-
-lemma gets_us_to_aux: "gets_us_to 1 drinks_before 1 <R 1 := d> p \<Longrightarrow> accepts drinks_before 1 <R 1 := d> p \<Longrightarrow>
-          posterior_sequence \<lbrakk>V (R 1) \<mapsto> cexp.Bc True, V (R 2) \<mapsto> cexp.Eq (Num 0)\<rbrakk> merge_1_2_update 1 <R 1 := d, R 2 := Num 0> p =
-          \<lbrakk>V (R 1) \<mapsto> cexp.Bc True, V (R 2) \<mapsto> cexp.Eq (Num 0)\<rbrakk>"
-proof (induct p)
-  case Nil
-  then show ?case
-  by simp
-next
-  case (Cons a p)
-  then show ?case
-    apply (case_tac a)
-    apply clarify
-    apply (simp del: posterior_sequence.simps)
-    apply (simp only: regsimp1 regsimp2 contextsimp1) \<comment> \<open>This makes it print nicely again\<close>
-    apply (rule gets_us_to.cases)
-       apply simp
-      apply simp
-     apply simp
-    apply clarify
-     apply (simp del: posterior_sequence.simps)
-     apply (simp add: stop_at_1)
-    apply clarify
-    apply simp
-    apply (case_tac "step merge_1_2_update 1 <R 1 := d, R 2 := Num 0> aa ba")
-     apply simp
-    apply simp
-    apply clarify
-    by (simp add: no_step_none)
-qed
-
-lemma accepts_trace_anterior: "accepts_trace drinks_before p \<Longrightarrow> gets_us_to 1 drinks_before 0 Map.empty p \<Longrightarrow> anterior_context merge_1_2_update p = \<lbrakk>V (R 1) \<mapsto> Bc True, V (R 2) \<mapsto> Eq (Num 0)\<rbrakk>"
-proof(induct p)
-  case Nil
-  then show ?case
-    apply simp
-    apply (rule gets_us_to.cases)
-    by auto
-next
-  have select_update_updates: "\<forall>ba. length ba = 1 \<longrightarrow> (EFSM.apply_updates (Updates select_update) (case_vname (\<lambda>n. input2state ba 1 (I n)) Map.empty) Map.empty) =
-        <R 1 := hd ba, R 2 := Num 0>"
-    apply clarify
+  have select_updates: "length b = 1 \<Longrightarrow> (EFSM.apply_updates (Updates select) (case_vname (\<lambda>n. input2state b 1 (I n)) Map.empty) Map.empty) = <R 1 := hd b>"
     apply (rule ext)
-    by (simp add: transitions hd_input2state)
-  case (Cons a p)
-  then show ?case
-    apply (case_tac a)
-    apply (case_tac "aa = ''select'' \<and> length b = 1")
-    defer
-     apply clarify
-     apply (rule gets_us_to.cases)
-        apply simp
-       apply simp
-    using drinks_before_step_0_invalid nondeterministic_step_none
-      apply auto[1]
-     apply simp
-
-    apply (rule gets_us_to.cases)
-       apply simp
+    by (simp add: hd_input2state select_def)
+  have select_update_updates: "length b = 1 \<Longrightarrow> (\<lambda>x. if x = R 1 then aval (snd (R 1, V (I 1))) (case_vname (\<lambda>n. input2state b 1 (I n)) Map.empty)
+          else EFSM.apply_updates [(R 2, L (Num 0))] (case_vname (\<lambda>n. input2state b 1 (I n)) Map.empty) Map.empty x) = <R 1 := hd b, R 2 := Num 0>"
+    apply (rule ext)
+    by (simp add: hd_input2state)
+  show ?thesis
+  apply (case_tac "aa = ''select'' \<and> length b = 1")
+     apply (rule nondeterministic_simulates_trace.step_some)
+         apply (simp add: update_before_def)
+        apply (simp add: nondeterministic_step_def possible_steps_drinks_before_select)
+       apply (simp add: nondeterministic_step_def possible_steps_merge_1_2_update_select transitions)
       apply simp
      defer
-     apply clarify
-     apply (simp add: step_def possible_steps_drinks_before_select)
+     apply (rule nondeterministic_simulates_trace.step_none)
+     apply (simp add: drinks_before_step_0_invalid)
+    apply (simp add: select_updates select_update_updates)
+    apply (case_tac t)
+     apply (simp add: nondeterministic_simulates_trace.base)
+    apply (case_tac a)
+    by (simp add: simulation_1_1)
+qed
 
-    apply clarify
-    apply (simp add: step_drinks_before_select)
-    apply clarify
-    apply (simp add: anterior_context_def step_def possible_steps_merge_1_2_update_select)
-    apply (simp add: accepts_trace_def)
-    apply (rule accepts.cases)
-      apply simp
-     apply simp
+lemma simulation_aux: "nondeterministic_simulates_trace (tm merge_1_2_update) (tm drinks_before) 0 0 Map.empty Map.empty t update_before"
+proof (induct t)
+case Nil
+  then show ?case
+    by (simp add: nondeterministic_simulates_trace.base)
+next
+  case (Cons a t)
+  then show ?case
+    apply (case_tac a)
     apply simp
-    apply clarify
-    apply (simp add: step_drinks_before_select)
-    apply clarify
-    apply (simp add: select_update_posterior select_update_updates)
-    by (simp add: gets_us_to_aux)
+    by (simp add: simulation_0_0)
 qed
 
-lemma coin_directly_subsumes_coin50: "directly_subsumes drinks_before merge_1_2_update 1 coin coin50"
-  apply (simp add: directly_subsumes_def)
-  apply clarify
-  by (simp add: accepts_trace_anterior coin_subsumes_coin50)
+lemma simulation: "nondeterministic_simulates (tm merge_1_2_update) (tm drinks_before) update_before"
+  apply (simp add:nondeterministic_simulates_def)
+  apply (rule allI)
+  by (simp add: simulation_aux)
 
-lemma step_merge_1_2_update_select: "step merge_1_2_update 0 Map.empty ''select'' [d] = Some (select_update, 1, [], <R 1 := d, R 2 := Num 0>)"
-  apply (simp add: step_def possible_steps_merge_1_2_update_select)
-  apply (simp add: transitions)
-  apply (rule ext)
-  by simp
-
-lemma step_merge_1_2_update_coin_50: "step merge_1_2_update 1 <R 1 := Str ''coke'', R 2 := Num 0> ''coin'' [Num 50] = None"
-  apply (simp add: step_def merge_1_2_update_possible_steps_coin_50 fis_singleton_def is_singleton_def)
-  by (simp add: transitions)
-
-lemma coin50_doesnt_subsume_coin: "\<not> subsumes \<lbrakk>V (R 1) \<mapsto> cexp.Bc True, V (R 2) \<mapsto> cexp.Eq (Num 0)\<rbrakk> coin50 coin"
+lemma "merge_transitions drinks_before merged_1_2 (leaves 2 drinks_before) (leaves 1 drinks_before) 1 1 1 coin 2 coin50 1 null_generator
+           (\<lambda>a b c d e. Some (merge_1_2_update, update_mapping, update_before)) True = Some a"
 proof-
-  have subsumption_violation: "(\<exists>r i. cval (medial \<lbrakk>V (R 1) \<mapsto> cexp.Bc True, V (R 2) \<mapsto> cexp.Eq (Num 0)\<rbrakk> (Guard coin) r) i = Some True \<and>
-           cval (medial \<lbrakk>V (R 1) \<mapsto> cexp.Bc True, V (R 2) \<mapsto> cexp.Eq (Num 0)\<rbrakk> (Guard coin50) r) i \<noteq> Some True)"
-    apply (simp add: transitions)
-    by auto
+  have leaves_1_drinks_before: "leaves 1 drinks_before = 1"
+  proof-
+    have set_filter: "Set.filter (\<lambda>x. \<exists>a b ba. x = (1, (a, b), ba)) (fset drinks_before) = {(1, (1, 2), coin50)}"
+      apply (simp add: Set.filter_def drinks_before_def)
+      apply safe
+      by (simp_all add: transitions)
+    show ?thesis
+      by (simp add: leaves_def ffilter_def fthe_elem_def Abs_fset_inverse set_filter)
+  qed
+  have leaves_2_coin_before: "leaves 2 drinks_before = 2"
+  proof-
+    have set_filter: "Set.filter (\<lambda>x. \<exists>a b ba. x = (2, (a, b), ba)) (fset drinks_before) = {(2, (2, 2), coin)}"
+      apply (simp add: Set.filter_def drinks_before_def)
+      apply safe
+      by (simp_all add: transitions)
+    show ?thesis
+      by (simp add: leaves_def ffilter_def fthe_elem_def Abs_fset_inverse set_filter)
+  qed
+  have easy_merge: "easy_merge drinks_before merged_1_2 (leaves 2 drinks_before) (leaves 1 drinks_before) 1 1 1 coin 2 coin50 1 null_generator = None"
+    apply (simp add: easy_merge_def null_generator_def leaves_1_drinks_before leaves_2_coin_before)
+    by (simp add: no_direct_subsumption_coin_coin50 no_direct_subsumption_coin50_coin)
   show ?thesis
-    by (simp add: subsumes_def subsumption_violation)
-qed
+    apply (simp add: merge_transitions_def easy_merge)
 
-lemma coin50_doesnt_directly_subsume_coin: "\<not> directly_subsumes drinks_before merge_1_2_update 2 coin50 coin"
+lemma "merge drinks_before 1 2 null_generator (\<lambda>a b c d e. Some (merge_1_2_update, update_mapping, update_before)) = Some merge_1_2_update"
+  apply (simp add: merge_def merge_states_1_2)
+  apply (simp add: nondeterminism_def nondeterministic_pairs_merged_1_2)
+
+
+lemma "infer drinks_before naive_score null_generator (\<lambda>a b c d e. Some (merge_1_2_update, update_mapping, update_before)) = drinks_after"
 proof-
   show ?thesis
-    apply (simp add: directly_subsumes_def)
-    apply (rule_tac x="[(''select'', [Str ''coke'']), (''coin'', [Num 50])]" in exI)
-    apply standard
-     apply (simp add: accepts_trace_def)
-     apply (rule accepts.step)
-      apply (simp add: step_drinks_before_select)
-     apply (rule accepts.step)
-      apply (simp add: step_drinks_before_coin_50)
-     apply (rule accepts.base)
-    apply standard
-    apply (rule gets_us_to.step_some)
-      apply (simp add: step_drinks_before_select)
-    apply (rule gets_us_to.step_some)
-      apply (simp add: step_drinks_before_coin_50)
-     apply (simp add: gets_us_to.base)
-    apply (simp add: anterior_context_def)
-    apply (simp add: step_merge_1_2_update_select step_merge_1_2_update_coin_50)
-    by (simp add: select_update_posterior coin50_doesnt_subsume_coin)
-qed
-
-lemma easy_merge_some: "easy_merge drinks_before merge_1_2_update 2 1 (update_mapping 1) (update_mapping 1) (update_mapping 1) coin coin50 (\<lambda>a b c d. Map.empty) =
-    Some drinks_after"
-proof-
-  have set_filter: "Set.filter (\<lambda>x. x \<noteq> ((1, 1), coin50)) (fset merge_1_2_update) = {((0, 1), select_update), ((1, 1), coin), ((1, 1), vend_fail), ((1, 3), vend_success)}"
-    apply (simp add: merge_1_2_update_def Set.filter_def)
-    apply safe
-    by (simp_all add: transitions)
-  have abs_fset: "Abs_fset {((0, 1), select_update), ((1, 1), coin), ((1, 1), vend_fail), ((1, 3), vend_success)} =
-                          {|((0, 1), select_update), ((1, 1), coin), ((1, 1), vend_fail), ((1, 3), vend_success)|}"
-    by (metis finsert.rep_eq fset_inverse fset_simps(1))
-  show ?thesis
-  apply (simp add: easy_merge_def coin_directly_subsumes_coin50 coin50_doesnt_directly_subsume_coin)
-    apply (simp add: replace_transition_def update_mapping_def ffilter_def set_filter abs_fset)
-    using drinks_after_def
-    by auto
-qed
-
-lemma merge_transitions: "merge_transitions drinks_before merge_1_2 2 1 1 1 1 coin coin50 (\<lambda>a b c d. Map.empty)
-                (\<lambda>a b c d e. Some (merge_1_2_update, update_mapping, update_before)) True = Some drinks_after"
-  apply (simp add: merge_transitions_def easy_merge_none)
-  by (simp add: simulation easy_merge_some)
-
-lemma "infer drinks_before naive_score (\<lambda>a b c d e. None) (\<lambda>a b c d e. Some (merge_1_2_update, update_mapping, update_before)) = drinks_after"
-proof-
-  have nondeterminism_merge_1_2: "nondeterminism merge_1_2"
-    by (simp add: nondeterminism_def nondeterministic_pairs)
-  show ?thesis
-    apply (simp add: score sorted_list_of_fset_def Let_def)
-    apply (simp add: merge_1_2 nondeterministic_pairs)
-    apply (simp add: coin_doesnt_exit_1_drinks_before coin50_exits_1_drinks_before)
-    apply (simp add: nondeterminism_merge_1_2)
-    apply (simp add: merge_transitions)
-    by (simp add: score_2)
+    apply (simp add: scoring_1)
 qed
 end
