michael_formal/Nondeterministic_EFSM.thy
@@ -9,6 +9,25 @@ definition nondeterministic_step :: "transition_matrix \<Rightarrow> nat \<Right
     Some (t, s', (apply_outputs (Outputs t) (join_ir i r)), (apply_updates (Updates t) (join_ir i r) r)))
   else None)"
 
+lemma fis_singleton_possible_steps: "fis_singleton (possible_steps e s r l i) \<Longrightarrow> \<exists>a b. (a, b) |\<in>| possible_steps e s r l i"
+  by (metis fempty_iff fset_eqI not_singleton_emty prod.exhaust_sel)
+
+lemma singleton_elem_eps: "is_singleton s \<Longrightarrow> the_elem s = x \<Longrightarrow> (SOME x. x \<in> s) = x"
+  by (simp add: is_singleton_the_elem)
+
+lemma step_nondet_step_equiv: "step e s r l i = Some t \<Longrightarrow> nondeterministic_step e s r l i = Some t"
+  apply (simp add: step_def nondeterministic_step_def)
+  apply (case_tac "fis_singleton (possible_steps e s r l i)")
+   apply (case_tac "fthe_elem (possible_steps e s r l i)")
+   apply simp
+   apply clarify
+   apply (case_tac "SOME x. x |\<in>| possible_steps e s r l i")
+   apply simp
+   apply (simp add: fis_singleton_possible_steps)
+   apply (simp add: fis_singleton_def fthe_elem_def fmember_def)
+   apply (simp add: singleton_elem_eps)
+  by simp
+
 primrec nondeterministic_observe_all :: "transition_matrix \<Rightarrow> nat \<Rightarrow> datastate \<Rightarrow> trace \<Rightarrow> (transition \<times> nat \<times> outputs \<times> datastate) list" where
   "nondeterministic_observe_all _ _ _ [] = []" |
   "nondeterministic_observe_all e s r (h#t) =
